thys/examples/sorting/Sorting_Introsort.thy
@@ -57,15 +57,6 @@ context weak_ordering begin
 
 end
 
-context sort_impl_context begin
-
-sepref_register introsort_aux4
-sepref_def introsort_aux_impl is "uncurry3 (PR_CONST introsort_aux4)" :: "(arr_assn)\<^sup>d *\<^sub>a size_assn\<^sup>k *\<^sub>a size_assn\<^sup>k *\<^sub>a size_assn\<^sup>k \<rightarrow>\<^sub>a arr_assn"
-  unfolding introsort_aux4_def PR_CONST_def
-  apply (annot_snat_const "TYPE(size_t)")
-  by sepref
-  
-  
 lemma introsort_depth_limit_in_bounds_aux: (* TODO: Move depth-computation into own (inline) function *)
   assumes "n < max_snat N" "1<N" shows "Discrete.log (n) * 2 < max_snat N"
 proof (cases "n=0")
@@ -81,6 +72,17 @@ next
     by (smt Suc_diff_Suc leI le_less_trans n_less_equal_power_2 nat_power_less_imp_less not_less_eq numeral_2_eq_2 numeral_2_eq_2 zero_order(3))
   ultimately show ?thesis .
 qed  
+  
+
+
+context sort_impl_context begin
+
+sepref_register introsort_aux4
+sepref_def introsort_aux_impl is "uncurry3 (PR_CONST introsort_aux4)" :: "(arr_assn)\<^sup>d *\<^sub>a size_assn\<^sup>k *\<^sub>a size_assn\<^sup>k *\<^sub>a size_assn\<^sup>k \<rightarrow>\<^sub>a arr_assn"
+  unfolding introsort_aux4_def PR_CONST_def
+  apply (annot_snat_const "TYPE(size_t)")
+  by sepref
+  
   
   
 sepref_register introsort4
@@ -99,6 +101,110 @@ theorem introsort_impl_correct: "(uncurry2 introsort_impl, uncurry2 (slice_sort_
   
   
 end
+
+
+
+context parameterized_weak_ordering begin
+  (* TODO: Move *)
+  lemmas heapsort_param_refine'[refine] = heapsort_param_refine[unfolded heapsort1.refine[OF WO.weak_ordering_axioms, symmetric]]
+  
+  
+  definition introsort_aux_param :: "'cparam \<Rightarrow> 'a list \<Rightarrow> nat \<Rightarrow> nat \<Rightarrow> nat \<Rightarrow> 'a list nres" where 
+    "introsort_aux_param cparam xs l h d \<equiv> RECT (\<lambda>introsort_aux (xs,l,h,d). doN {
+    ASSERT (l\<le>h);
+    if h-l > is_threshold then doN {
+      if d=0 then
+        heapsort_param cparam xs l h
+      else doN {
+        (xs,m)\<leftarrow>partition_pivot_param cparam xs l h;
+        xs \<leftarrow> introsort_aux (xs,l,m,d-1);
+        xs \<leftarrow> introsort_aux (xs,m,h,d-1);
+        RETURN xs
+      }
+    }
+    else
+      RETURN xs
+  }) (xs,l,h,d)"
+
+
+  lemma introsort_aux_param_refine[refine]: 
+    "\<lbrakk> (xs',xs)\<in>cdom_list_rel cparam; (l',l)\<in>Id; (h',h)\<in>Id; (d',d)\<in>Id
+    \<rbrakk> \<Longrightarrow> introsort_aux_param cparam xs' l' h' d' \<le>\<Down>(cdom_list_rel cparam) (WO.introsort_aux4 cparam xs l h d)"
+    unfolding introsort_aux_param_def WO.introsort_aux4_def 
+    supply [refine_dref_RELATES] = RELATESI[of "cdom_list_rel cparam"]
+    apply (refine_rcg)
+    apply refine_dref_type
+    apply simp_all 
+    done
+
+  definition "introsort_param cparam xs l h \<equiv> doN {
+    ASSERT(l\<le>h);
+    if h-l>1 then doN {
+      xs \<leftarrow> introsort_aux_param cparam xs l h (Discrete.log (h-l)*2);
+      xs \<leftarrow> final_insertion_sort_param cparam xs l h;
+      RETURN xs
+    } else RETURN xs
+  }"  
+
+  lemma introsort_param_refine: 
+    "\<lbrakk> (xs',xs)\<in>cdom_list_rel cparam; (l',l)\<in>Id; (h',h)\<in>Id
+    \<rbrakk> \<Longrightarrow> introsort_param cparam xs' l' h' \<le> \<Down>(cdom_list_rel cparam) (WO.introsort4 cparam xs l h)"
+    unfolding introsort_param_def WO.introsort4_def
+    apply (refine_rcg)
+    by auto
+
+      
+  lemma introsort_param_correct: 
+    assumes "(xs',xs)\<in>Id" "(l',l)\<in>Id" "(h',h)\<in>Id"
+    shows "introsort_param cparam xs' l' h' \<le> pslice_sort_spec cdom pless cparam xs l h"
+  proof -
+    note introsort_param_refine
+    also note WO.introsort4_correct
+    also note slice_sort_spec_xfer
+    finally show ?thesis 
+      unfolding pslice_sort_spec_def
+      apply refine_vcg
+      using assms unfolding cdom_list_rel_alt
+      by (simp add: in_br_conv)
+    
+  qed
+  
+  lemma introsort_param_correct': 
+    shows "(PR_CONST introsort_param, PR_CONST (pslice_sort_spec cdom pless)) \<in> Id \<rightarrow> Id \<rightarrow> Id \<rightarrow> Id \<rightarrow> \<langle>Id\<rangle>nres_rel"
+    using introsort_param_correct 
+    apply (intro fun_relI nres_relI) 
+    by simp
+  
+    
+    
+    
+end
+
+context parameterized_sort_impl_context begin
+
+
+sepref_register introsort_aux_param
+sepref_def introsort_aux_param_impl is "uncurry4 (PR_CONST introsort_aux_param)" 
+  :: "cparam_assn\<^sup>k *\<^sub>a (arr_assn)\<^sup>d *\<^sub>a size_assn\<^sup>k *\<^sub>a size_assn\<^sup>k *\<^sub>a size_assn\<^sup>k \<rightarrow>\<^sub>a arr_assn"
+  unfolding introsort_aux_param_def PR_CONST_def
+  apply (annot_snat_const "TYPE(size_t)")
+  by sepref
+  
+  
+sepref_register introsort_param
+sepref_def introsort_param_impl is "uncurry3 (PR_CONST introsort_param)" :: "cparam_assn\<^sup>k *\<^sub>a (arr_assn)\<^sup>d *\<^sub>a size_assn\<^sup>k *\<^sub>a size_assn\<^sup>k \<rightarrow>\<^sub>a arr_assn"
+  unfolding introsort_param_def PR_CONST_def
+  apply (annot_snat_const "TYPE(size_t)")
+  supply [intro!] = introsort_depth_limit_in_bounds_aux 
+  by sepref
+
+
+lemma introsort_param_impl_correct: "(uncurry3 introsort_param_impl, uncurry3 (PR_CONST (pslice_sort_spec cdom pless)))
+        \<in> cparam_assn\<^sup>k *\<^sub>a arr_assn\<^sup>d *\<^sub>a snat_assn\<^sup>k *\<^sub>a snat_assn\<^sup>k \<rightarrow>\<^sub>a arr_assn"
+  using introsort_param_impl.refine[FCOMP introsort_param_correct'] .
+  
+end
+
 
  (* TODO: Move! *)
 lemmas [llvm_inline] = 
@@ -183,7 +289,6 @@ definition llstrcmp :: "(8 word,size_t)array_list ptr \<Rightarrow> _ \<Rightarr
     r \<leftarrow> strcmp_impl a b;
     if r\<noteq>0 then return 1 else return 0
   }"
-  
   
 export_llvm 
   "unat_sort_introsort_impl :: 64 word ptr \<Rightarrow> _" is "uint64_t* introsort(uint64_t*, int64_t, int64_t)" 
