thys/examples/sorting/Sorting_Quicksort_Partition.thy
@@ -341,5 +341,197 @@ sepref_def partition_pivot_impl [llvm_inline] is "uncurry2 (PR_CONST partition_p
 
 end
 
+
+subsection \<open>Parameterization\<close>
+
+context parameterized_weak_ordering begin
+  thm WO.qsp_next_l_def
+
+  definition qsp_next_l_param :: "'cparam \<Rightarrow> 'a list \<Rightarrow> nat \<Rightarrow> nat \<Rightarrow> nat \<Rightarrow> nat nres" where            
+    "qsp_next_l_param cparam xs pi li hi \<equiv> doN {
+      monadic_WHILEIT (\<lambda>_. True) 
+        (\<lambda>li. doN {ASSERT (li\<noteq>pi); pcmp_idxs2 cparam xs li pi}) 
+        (\<lambda>li. doN {ASSERT (li<hi); RETURN (li + 1)}) li
+    }"  
+  
+  lemma qsp_next_l_param_refine[refine]: "\<lbrakk>
+    (xs',xs)\<in>cdom_list_rel cparam; (p',p)\<in>Id; (i',i)\<in>Id; (h',h)\<in>Id
+  \<rbrakk> \<Longrightarrow> qsp_next_l_param cparam xs' p' i' h' \<le>\<Down>nat_rel (WO.ungrd_qsp_next_l_spec cparam xs p i h)"
+  proof (goal_cases)
+    case 1
+    then have "qsp_next_l_param cparam xs' p' i' h' \<le>\<Down>nat_rel (WO.qsp_next_l cparam xs p i h)" 
+      unfolding qsp_next_l_param_def WO.qsp_next_l_def
+      apply refine_rcg
+      by auto
+    also note WO.qsp_next_l_refine[param_fo, OF IdI IdI IdI IdI, of cparam xs p i h, THEN nres_relD]
+    finally show ?case unfolding PR_CONST_def .
+  qed 
+  
+    
+  definition qsp_next_h_param :: "'cparam \<Rightarrow> 'a list \<Rightarrow> nat \<Rightarrow> nat \<Rightarrow> nat nres" where
+    "qsp_next_h_param cparam xs pi hi \<equiv> doN {
+      ASSERT (hi>0);
+      let hi = hi - 1;
+      ASSERT (hi<length xs);
+      monadic_WHILEIT (\<lambda>_. True)
+        (\<lambda>hi. doN {ASSERT(pi\<noteq>hi); pcmp_idxs2 cparam xs pi hi}) 
+        (\<lambda>hi. doN { ASSERT(hi>0); RETURN (hi - 1)}) hi
+    }"  
+
+  lemma qsp_next_h_param_refine[refine]: "\<lbrakk>
+    (xs',xs)\<in>cdom_list_rel cparam; (p',p)\<in>Id; (h',h)\<in>Id
+  \<rbrakk> \<Longrightarrow> qsp_next_h_param cparam xs' p' h' \<le>\<Down>nat_rel (WO.ungrd_qsp_next_h_spec cparam xs p h)"      
+  proof goal_cases
+    case 1
+    then have "qsp_next_h_param cparam xs' p' h' \<le>\<Down>nat_rel (WO.qsp_next_h cparam xs p h)"
+      unfolding qsp_next_h_param_def WO.qsp_next_h_def
+      apply refine_rcg
+      by (auto simp: cdom_list_rel_alt in_br_conv)
+    also note WO.qsp_next_h_refine[param_fo, THEN nres_relD]
+    finally show ?thesis by simp 
+  qed    
+    
+  definition "qs_partition_param cparam li\<^sub>0 hi\<^sub>0 pi xs\<^sub>0 \<equiv> doN {
+    ASSERT (pi < li\<^sub>0 \<and> li\<^sub>0<hi\<^sub>0 \<and> hi\<^sub>0\<le>length xs\<^sub>0);
+    
+    \<comment> \<open>Initialize\<close>
+    li \<leftarrow> qsp_next_l_param cparam xs\<^sub>0 pi li\<^sub>0 hi\<^sub>0;
+    hi \<leftarrow> qsp_next_h_param cparam xs\<^sub>0 pi hi\<^sub>0;
+    
+    ASSERT (li\<^sub>0\<le>hi);
+    
+    (xs,li,hi) \<leftarrow> WHILEIT 
+      (\<lambda>_. True)
+      (\<lambda>(xs,li,hi). li<hi) 
+      (\<lambda>(xs,li,hi). doN {
+        ASSERT(li<hi \<and> li<length xs \<and> hi<length xs \<and> li\<noteq>hi);
+        xs \<leftarrow> mop_list_swap xs li hi;
+        let li = li + 1;
+        li \<leftarrow> qsp_next_l_param cparam xs pi li hi\<^sub>0;
+        hi \<leftarrow> qsp_next_h_param cparam xs pi hi;
+        RETURN (xs,li,hi)
+      }) 
+      (xs\<^sub>0,li,hi);
+    
+    RETURN (xs,li)
+  }"  
+
+  lemma qs_partition_param_refine[refine]: "\<lbrakk>
+    (li',li)\<in>Id; (hi',hi)\<in>Id; (pi',pi)\<in>Id; (xs',xs)\<in>cdom_list_rel cparam
+  \<rbrakk> \<Longrightarrow> qs_partition_param cparam li' hi' pi' xs' 
+    \<le> \<Down>(cdom_list_rel cparam \<times>\<^sub>r nat_rel) (WO.qs_partition cparam li hi pi xs)" 
+    unfolding qs_partition_param_def WO.qs_partition_def
+    supply [refine_dref_RELATES] = RELATESI[of "cdom_list_rel cparam"]
+    apply refine_rcg
+    apply refine_dref_type
+    apply (auto simp: cdom_list_rel_alt in_br_conv)
+    done
+
+ definition "move_median_to_first_param cparam ri ai bi ci (xs::'a list) = doN {
+    ASSERT (ai \<noteq> bi \<and> ai \<noteq> ci \<and> bi \<noteq> ci \<and> ri \<noteq> ai \<and> ri \<noteq> bi \<and> ri \<noteq> ci);
+    if\<^sub>N pcmp_idxs2 cparam xs ai bi then (
+      if\<^sub>N pcmp_idxs2 cparam xs bi ci then
+        mop_list_swap xs ri bi
+      else if\<^sub>N pcmp_idxs2 cparam xs ai ci then
+        mop_list_swap xs ri ci
+      else 
+        mop_list_swap xs ri ai
+    ) 
+    else if\<^sub>N pcmp_idxs2 cparam xs ai ci then
+      mop_list_swap xs ri ai
+    else if\<^sub>N pcmp_idxs2 cparam xs bi ci then 
+      mop_list_swap xs ri ci
+    else 
+      mop_list_swap xs ri bi
+  }"
+
+  
+  (* TODO:Move *)
+  lemma mop_list_swap_cdom_refine[refine]: "\<lbrakk>
+    (xs',xs)\<in>cdom_list_rel cparam; (i',i)\<in>Id; (j',j)\<in>Id
+  \<rbrakk> \<Longrightarrow> mop_list_swap xs' i' j' \<le> \<Down> (cdom_list_rel cparam) (mop_list_swap xs i j)"
+    apply simp
+    apply refine_rcg
+    apply (clarsimp_all simp: cdom_list_rel_def list_rel_imp_same_length)
+    apply (parametricity)
+    by auto
+  
+  lemma move_median_to_first_param_refine[refine]: "\<lbrakk>
+    (ri',ri)\<in>Id; (ai',ai)\<in>Id; (bi',bi)\<in>Id; (ci',ci)\<in>Id; (xs',xs)\<in>cdom_list_rel cparam 
+  \<rbrakk> \<Longrightarrow> move_median_to_first_param cparam ri' ai' bi' ci' xs' 
+    \<le> \<Down>(cdom_list_rel cparam) (WO.move_median_to_first cparam ri ai bi ci xs)"
+    unfolding move_median_to_first_param_def WO.move_median_to_first_alt
+    apply refine_rcg  
+    by auto  
+    
+  definition "partition_pivot_param cparam xs\<^sub>0 l h \<equiv> doN {
+    ASSERT (l\<le>h \<and> h\<le>length xs\<^sub>0 \<and> h-l\<ge>4);
+    let m = l + (h-l) div 2;
+    xs\<^sub>1 \<leftarrow> move_median_to_first_param cparam l (l+1) m (h-1) xs\<^sub>0;
+    ASSERT (l<length xs\<^sub>1 \<and> length xs\<^sub>1 = length xs\<^sub>0);
+    (xs,m) \<leftarrow> qs_partition_param cparam (l+1) h l xs\<^sub>1;
+  
+    RETURN (xs,m)
+  }"
+
+  lemma partition_pivot_param_refine[refine]: "\<lbrakk> (xs',xs)\<in>cdom_list_rel cparam; (l',l)\<in>Id; (h',h)\<in>Id
+    \<rbrakk> \<Longrightarrow> partition_pivot_param cparam xs' l' h' 
+        \<le> \<Down>(cdom_list_rel cparam \<times>\<^sub>r nat_rel) (WO.partition_pivot cparam xs l h)"
+    unfolding partition_pivot_param_def WO.partition_pivot_def   
+    apply refine_rcg
+    apply (auto simp: cdom_list_rel_alt in_br_conv)
+    done    
+        
+end
+
+
+context parameterized_sort_impl_context begin
+
+  (* TODO: Move *)
+  abbreviation "arr_assn \<equiv> woarray_assn elem_assn"
+
+  
+sepref_register qsp_next_l_param qsp_next_h_param
+
+(* TODO: We can get rid of the length xs restriction: the stopper element will always lie within <h, which is size_t representable! *)
+sepref_def qsp_next_l_impl [llvm_inline] is "uncurry4 (PR_CONST qsp_next_l_param)" 
+  :: "cparam_assn\<^sup>k *\<^sub>a (arr_assn)\<^sup>k *\<^sub>a size_assn\<^sup>k *\<^sub>a size_assn\<^sup>k *\<^sub>a size_assn\<^sup>k \<rightarrow>\<^sub>a size_assn"
+  unfolding qsp_next_l_param_def PR_CONST_def
+  apply (annot_snat_const "TYPE(size_t)")
+  by sepref
+ 
+sepref_def qsp_next_h_impl [llvm_inline] is "uncurry3 (PR_CONST qsp_next_h_param)" :: "cparam_assn\<^sup>k *\<^sub>a (arr_assn)\<^sup>k *\<^sub>a size_assn\<^sup>k *\<^sub>a size_assn\<^sup>k \<rightarrow>\<^sub>a size_assn"
+  unfolding qsp_next_h_param_def PR_CONST_def
+  apply (annot_snat_const "TYPE(size_t)")
+  by sepref
+  
+                        
+sepref_register qs_partition_param  
+sepref_def qs_partition_impl is "uncurry4 (PR_CONST qs_partition_param)" :: "cparam_assn\<^sup>k *\<^sub>a size_assn\<^sup>k *\<^sub>a size_assn\<^sup>k *\<^sub>a size_assn\<^sup>k *\<^sub>a (arr_assn)\<^sup>d \<rightarrow>\<^sub>a arr_assn \<times>\<^sub>a size_assn"
+  unfolding qs_partition_param_def PR_CONST_def
+  apply (annot_snat_const "TYPE(size_t)")
+  supply [dest] = slice_eq_mset_eq_length
+  by sepref
+
+sepref_register move_median_to_first_param
+
+sepref_def move_median_to_first_param_impl [llvm_inline] 
+  is "uncurry5 (PR_CONST move_median_to_first_param)" 
+  :: "cparam_assn\<^sup>k *\<^sub>a size_assn\<^sup>k *\<^sub>a size_assn\<^sup>k *\<^sub>a size_assn\<^sup>k *\<^sub>a size_assn\<^sup>k *\<^sub>a (arr_assn)\<^sup>d \<rightarrow>\<^sub>a arr_assn"
+  unfolding move_median_to_first_param_def PR_CONST_def
+  by sepref  
+  
+  
+sepref_register partition_pivot_param  
+sepref_def partition_pivot_impl [llvm_inline] 
+  is "uncurry3 (PR_CONST partition_pivot_param)" 
+  :: "cparam_assn\<^sup>k *\<^sub>a arr_assn\<^sup>d *\<^sub>a size_assn\<^sup>k *\<^sub>a size_assn\<^sup>k \<rightarrow>\<^sub>a arr_assn \<times>\<^sub>a size_assn"
+  unfolding partition_pivot_param_def PR_CONST_def    
+  apply (annot_snat_const "TYPE(size_t)")
+  by sepref
+  
+
+end
+
 end                           
 
